add lfp and gfp definition

eIris/tests/inductive.v
@@ -2,10 +2,10 @@ From elpi Require Import elpi.
 From iris.proofmode Require Import proofmode tactics coq_tactics reduction.
 From iris.prelude Require Import options.
 From iris.bi Require Import fixpoint.
-From iris.algebra Require Import list.
+From iris.algebra Require Import ofe monoid list.
 From iris.heap_lang Require Import proofmode.
 From iris.heap_lang Require Import notation.
-From stdpp Require Import base.
+From stdpp Require Import base finite.
 
 Context `{!heapGS Σ}.
 Notation iProp := (iProp Σ).
@@ -29,6 +29,11 @@ Proof.
 Qed.
 
 Definition is_list_def := fixpoint is_list_pre.
+
+Lemma is_list_def_unfold hd vs :
+    is_list_def hd vs ⊣⊢ is_list_pre is_list_def hd vs.
+Proof. apply (fixpoint_unfold is_list_pre). Qed.
+
 
 Definition is_list_pre_lgfp (is_list : val → list val → iProp) : val → list val → iProp := λ hd vs,
   match vs with
@@ -64,12 +69,113 @@ Proof.
     iApply is_list_pre_lgfp_mono.
     iIntros "!>" (hd vs).
     iApply "H".
-  - intros is_list Hne n [hd vs] [hd' vs'] [? ?]; simplify_eq /=.
+  - intros is_list Hne n [hd vs] [hd' vs'] [Hhd Hvs]; simplify_eq /=.
     rewrite /curry /is_list_pre_lgfp.
-    f_equiv.
-    destruct vs.
-    + 
+    revert Hvs; revert vs'.
+    induction vs as [|v vs IH]; intros vs' Hvs; setoid_rewrite list_dist_Forall2 in Hvs. 
+    + apply Forall2_nil_inv_l in Hvs. 
+      simplify_eq. 
+      setoid_rewrite Hhd.
+      f_equiv.
+    + inversion Hvs; simplify_eq /=.
+      setoid_rewrite H1.
+      setoid_rewrite Hhd.
+      repeat f_equiv.
+      by apply list_dist_Forall2.
+Qed.
 
-Definition is_list_lfp_def := bi_least_fixpoint 
+Definition is_list_lfp_def := λ hd vs, bi_least_fixpoint is_list_pre_lgfp' (hd, vs).
+Definition is_list_gfp_def := λ hd vs, bi_greatest_fixpoint is_list_pre_lgfp' (hd, vs).
 
+Lemma is_list_lfp_unfold hd vs :
+  is_list_lfp_def hd vs ⊣⊢ is_list_pre_lgfp is_list_lfp_def hd vs.
+Proof. by rewrite /is_list_lfp_def least_fixpoint_unfold. Qed.
 
+Lemma is_list_gfp_unfold hd vs :
+  is_list_gfp_def hd vs ⊣⊢ is_list_pre_lgfp is_list_gfp_def hd vs.
+Proof. by rewrite /is_list_gfp_def greatest_fixpoint_unfold. Qed.
+
+Section Proofs.
+  Definition app : val :=
+    rec: "app" "l" "l'" :=
+      match: "l" with
+        NONE => "l'"
+      | SOME "hd" =>
+        let: "tmp1" := !"hd" in
+        let: "tmp2" := "app" (Snd "tmp1") "l'" in
+        "hd" <- ((Fst "tmp1"), "tmp2");;
+            "l"
+      end.
+
+  Definition cons : val := (λ: "x" "xs",
+    let: "p" := ("x", "xs") in
+    SOME (Alloc("p"))).
+
+  Definition empty_list : val := NONEV.
+
+  Lemma app_spec_fix xs ys (l l' : val) :
+  {{{ is_list_fix l xs ∗ is_list_fix l' ys }}}
+    app l l'
+  {{{ v, RET v; is_list_fix v (xs ++ ys) }}}.
+  Proof.
+    iIntros (ϕ) "[Hxs Hys] H".
+    iLöb as "IH" forall (l xs l' ys ϕ).
+    destruct xs as [| x xs']; iSimplifyEq.
+    - wp_rec. wp_let. wp_match. iApply "H". done.
+    - iDestruct "Hxs" as (l0 hd0) "(% & Hx & Hxs)". iSimplifyEq.
+      wp_rec. wp_let. wp_match. wp_load. wp_let. wp_proj. wp_bind (app _ _)%E.
+      iApply ("IH" with "Hxs Hys").
+      iNext. iIntros (v) "?". wp_let. wp_proj. wp_store. iSimplifyEq. iApply "H".
+      iExists l0, _. iFrame. done.
+  Qed.
+
+  Lemma app_spec_banach xs ys (l l' : val) :
+  {{{ is_list_def l xs ∗ is_list_def l' ys }}}
+    app l l'
+  {{{ v, RET v; is_list_def v (xs ++ ys) }}}.
+  Proof.
+    iIntros (ϕ) "[Hxs Hys] H".
+    iLöb as "IH" forall (l xs l' ys ϕ).
+    destruct xs as [| x xs']; rewrite is_list_def_unfold; iSimplifyEq.
+    - wp_rec. wp_let. wp_match. iApply "H". done.
+    - iDestruct "Hxs" as (l0 hd0) "(% & Hx & Hxs)". iSimplifyEq.
+      wp_rec. wp_let. wp_match. wp_load. wp_let. wp_proj. wp_bind (app _ _)%E.
+      iApply ("IH" with "Hxs Hys").
+      iNext. iIntros (v) "?". wp_let. wp_proj. wp_store. iSimplifyEq. iApply "H".
+      iApply is_list_def_unfold. simpl.
+      iExists l0, _. iFrame. done.
+  Qed.
+
+  Lemma app_spec_lfp xs ys (l l' : val) :
+  {{{ is_list_lfp_def l xs ∗ is_list_lfp_def l' ys }}}
+    app l l'
+  {{{ v, RET v; is_list_lfp_def v (xs ++ ys) }}}.
+  Proof.
+    iIntros (ϕ) "[Hxs Hys] H".
+    iLöb as "IH" forall (l xs l' ys ϕ).
+    destruct xs as [| x xs']; rewrite is_list_lfp_unfold; iSimplifyEq.
+    - wp_rec. wp_let. wp_match. iApply "H". done.
+    - iDestruct "Hxs" as (l0 hd0) "(% & Hx & Hxs)". iSimplifyEq.
+      wp_rec. wp_let. wp_match. wp_load. wp_let. wp_proj. wp_bind (app _ _)%E.
+      iApply ("IH" with "Hxs Hys").
+      iNext. iIntros (v) "?". wp_let. wp_proj. wp_store. iSimplifyEq. iApply "H".
+      iApply is_list_lfp_unfold. simpl.
+      iExists l0, _. iFrame. done.
+  Qed.
+
+  Lemma app_spec_gfp xs ys (l l' : val) :
+  {{{ is_list_gfp_def l xs ∗ is_list_gfp_def l' ys }}}
+    app l l'
+  {{{ v, RET v; is_list_gfp_def v (xs ++ ys) }}}.
+  Proof.
+    iIntros (ϕ) "[Hxs Hys] H".
+    iLöb as "IH" forall (l xs l' ys ϕ).
+    destruct xs as [| x xs']; rewrite is_list_gfp_unfold; iSimplifyEq.
+    - wp_rec. wp_let. wp_match. iApply "H". done.
+    - iDestruct "Hxs" as (l0 hd0) "(% & Hx & Hxs)". iSimplifyEq.
+      wp_rec. wp_let. wp_match. wp_load. wp_let. wp_proj. wp_bind (app _ _)%E.
+      iApply ("IH" with "Hxs Hys").
+      iNext. iIntros (v) "?". wp_let. wp_proj. wp_store. iSimplifyEq. iApply "H".
+      iApply is_list_gfp_unfold. simpl.
+      iExists l0, _. iFrame. done.
+  Qed.
